Let's tackle each part of the problem systematically:

### Part (a): Compute $ p_{y_0} = P(Y = 0) $

We need to calculate the probability that the output $ Y $ is 0, which can happen if:

1. $ X = 0 $ and there is no error (probability $ 1 - p $),
2. $ X = 1 $ and there is an error (probability $ 2p $).

Given that $ P(X = 0) = \pi_0 $ and $ P(X = 1) = 1 - \pi_0 $, we can compute $ P(Y = 0) $ as follows:

$p_{y_0} = P(Y = 0) = P(Y = 0 | X = 0) \cdot P(X = 0) + P(Y = 0 | X = 1) \cdot P(X = 1)$
Substitute the given values:
$p_{y_0} = (1 - p) \cdot \pi_0 + 2p \cdot (1 - \pi_0)$
Expanding and simplifying, we get:
$p_{y_0} = \pi_0 - \pi_0 \cdot p + 2p - 2p \cdot \pi_0 = \pi_0(1 - 3p) + 2p$

### Part (b): Formula for $ I(X, Y) $

The mutual information $ I(X, Y) $ can be written in terms of entropy as:
$I(X, Y) = H(Y) - H(Y | X)$

Using the binary entropy function $ \varphi(x) = -x \ln x - (1 - x) \ln (1 - x) $, we will express $ H(Y) $ and $ H(Y | X) $ in terms of $ \varphi $.

1. **Calculate $ H(Y) $:**

   Since $ Y $ is binary, $ H(Y) = \varphi(p_{y_0}) $, where $ p_{y_0} $ was computed in part (a).

2. **Calculate $ H(Y | X) $:**

   The conditional entropy $ H(Y | X) $ is calculated as:
   $   H(Y | X) = P(X = 0) H(Y | X = 0) + P(X = 1) H(Y | X = 1)
$
   - When $ X = 0 $: $ Y = 0 $ with probability $ 1 - p $ and $ Y = 1 $ with probability $ p $, so $ H(Y | X = 0) = \varphi(p) $.
   - When $ X = 1 $: $ Y = 0 $ with probability $ 2p $ and $ Y = 1 $ with probability $ 1 - 2p $, so $ H(Y | X = 1) = \varphi(2p) $.

   Thus,
   $   H(Y | X) = \pi_0 \varphi(p) + (1 - \pi_0) \varphi(2p)
$

Now, combining terms:
$I(X, Y) = \varphi(p_{y_0}) - \pi_0 \varphi(p) - (1 - \pi_0) \varphi(2p)$

This can be expressed in the form given:
$I(X, Y) = \varphi(a) + b \varphi(p) + c \varphi(2p)$
where:
- $ a = p_{y_0} = \pi_0(1 - 3p) + 2p $,
- $ b = -\pi_0 $,
- $ c = -(1 - \pi_0) $.

### Part (c): Formula for the derivative of the binary entropy function, $ \varphi'(x) $

The binary entropy function is:
$\varphi(x) = -x \ln x - (1 - x) \ln(1 - x)$

Taking the derivative with respect to $ x $:
$\varphi'(x) = -\ln x + \ln(1 - x)$

### Part (d): Determine which variable to differentiate with respect to for channel capacity

To find the channel capacity, we maximize the mutual information $ I(X, Y) $ with respect to the input distribution $ \pi_0 $. This is done by setting $ \partial I / \partial \pi_0 = 0 $.

### Part (e): Set up the equation for finding the channel capacity

$\frac{\partial I}{\partial \pi_0} = 0$
$\frac{\partial I}{\partial \pi_0} = \frac{\partial \varphi(p_{y_0})}{\partial p_{y_0}} \cdot \frac{\partial p_{y_0}}{\partial \pi_0} - \varphi(p) + \varphi(2p) = 0$
where
$\frac{\partial \varphi(p_{y_0})}{\partial p_{y_0}} = \varphi'(p_{y_0})$,
$\frac{\partial p_{y_0}}{\partial \pi_0} = 1 - 3p$.
Thus, the equation becomes:
$\varphi'(p_{y_0}) (1 - 3p) - \varphi(p) + \varphi(2p) = 0$
expands into

This is the equation you would set up to solve for the channel capacity, but no further simplification or solving is required as per the problem statement.
To expand part (e) in terms of \( p \), let's recall the expression we derived for the channel capacity condition:

\[
\frac{\partial I}{\partial \pi_0} = 0
\]

which gives us the following condition:

\[
\varphi'(p_{y_0}) (1 - 3p) - \varphi(p) + \varphi(2p) = 0
\]

where:
- \( \varphi(x) \) is the binary entropy function, given by \( \varphi(x) = -x \ln x - (1 - x) \ln(1 - x) \),
- \( p_{y_0} = \pi_0 (1 - 3p) + 2p \) is the probability of \( Y = 0 \).

### Step-by-Step Expansion

1. **Compute \( \varphi'(p_{y_0}) \):**

   The derivative of the binary entropy function \( \varphi(x) \) is:
   \[
   \varphi'(x) = -\ln x + \ln(1 - x)
   \]

   Substituting \( x = p_{y_0} \), we have:
   \[
   \varphi'(p_{y_0}) = -\ln(p_{y_0}) + \ln(1 - p_{y_0})
   \]

2. **Express \( p_{y_0} \) in terms of \( p \):**

   Recall that:
   \[
   p_{y_0} = \pi_0 (1 - 3p) + 2p
   \]

3. **Expand the equation:**

   Substitute \( \varphi'(p_{y_0}) \) and the expression for \( p_{y_0} \) into the capacity condition:

   \[
   [-\ln(\pi_0 (1 - 3p) + 2p) + \ln(1 - (\pi_0 (1 - 3p) + 2p))] (1 - 3p) - \varphi(p) + \varphi(2p) = 0
   \]

4. **Express \( \varphi(p) \) and \( \varphi(2p) \):**

   Using the definition of \( \varphi(x) \):
   \[
   \varphi(p) = -p \ln p - (1 - p) \ln(1 - p)
   \]
   and
   \[
   \varphi(2p) = -2p \ln(2p) - (1 - 2p) \ln(1 - 2p)
   \]

5. **Final expanded form:**

   Substitute these expressions for \( \varphi(p) \) and \( \varphi(2p) \) into the capacity condition equation:

$\ln\frac{1 - (\pi_0 (1 - 3p) + 2p)}{(\pi_0 (1 - 3p) + 2p)} (1 - 3p)$
$- [-p \ln p - (1 - p) \ln(1 - p)]$
$+ [-2p \ln(2p) - (1 - 2p) \ln(1 - 2p)] = 0$

This is the expanded form of the equation for finding the channel capacity by setting \( \partial I / \partial \pi_0 = 0 \). Solving this equation explicitly would require numerical methods, as it does not simplify easily into a closed form.